rt refine: sketch out sched context invocations
Signed-off-by: Gerwin Klein <gerwin.klein@data61.csiro.au>

proof/refine/ARM/SchedContextInv_R.thy
@@ -10,6 +10,83 @@ begin
 
 context begin interpretation Arch . (*FIXME: arch_split*)
 
+primrec valid_sc_inv' :: "sched_context_invocation \<Rightarrow> kernel_state \<Rightarrow> bool" where
+  "valid_sc_inv' (InvokeSchedContextConsumed scptr args) = (sc_at' scptr and ex_nonz_cap_to' scptr)"
+| "valid_sc_inv' (InvokeSchedContextBind scptr cap) =
+     (ex_nonz_cap_to' scptr and valid_cap' cap and
+        (case cap of
+           ThreadCap t \<Rightarrow>
+             ex_nonz_cap_to' t and
+             bound_sc_tcb_at' ((=) None) t and
+             obj_at' (\<lambda>sc. scTCB sc = None) scptr \<^cancel>\<open> and
+             FIXME RT: can hopefully be established via assertions:
+             (\<lambda>s. st_tcb_at' (ipc_queued_thread_state) t s
+                     \<longrightarrow> sc_at_pred' (sc_released (cur_time s)) scptr s) \<close>
+         | NotificationCap n _ _ _ \<Rightarrow>
+             ex_nonz_cap_to' n and
+             obj_at' (\<lambda>ntfn. ntfnSc ntfn = None) n and
+             obj_at' (\<lambda>sc. scNtfn sc = None) scptr
+         | _ \<Rightarrow> \<bottom>))"
+| "valid_sc_inv' (InvokeSchedContextUnbindObject scptr cap) =
+     (ex_nonz_cap_to' scptr and valid_cap' cap and
+        (case cap of
+           ThreadCap t \<Rightarrow>
+             ex_nonz_cap_to' t and obj_at' (\<lambda>sc. scTCB sc = Some t) scptr and
+             (\<lambda>s. t \<noteq> ksCurThread s)
+         | NotificationCap n _ _ _ \<Rightarrow>
+             ex_nonz_cap_to' n and obj_at' (\<lambda>sc. scNtfn sc = Some n) scptr
+         | _ \<Rightarrow> \<bottom>))"
+| "valid_sc_inv' (InvokeSchedContextUnbind scptr) = (sc_at' scptr and ex_nonz_cap_to' scptr)"
+| "valid_sc_inv' (InvokeSchedContextYieldTo scptr args) =
+     (\<lambda>s. ex_nonz_cap_to' scptr s \<and>
+          (\<forall>ct. ct = ksCurThread s \<longrightarrow>
+                bound_yt_tcb_at' ((=) None) ct s \<and>
+                obj_at' (\<lambda>sc. \<exists>t. scTCB sc = Some t \<and> t \<noteq> ct) scptr s))"
+
+(* FIXME RT: valid_refills_number is probably wrong for Haskell *)
+primrec valid_sc_ctrl_inv' :: "sched_control_invocation \<Rightarrow> kernel_state \<Rightarrow> bool" where
+  "valid_sc_ctrl_inv' (InvokeSchedControlConfigure scptr budget period mrefills badge) =
+     ((\<lambda>s. \<exists>n. sc_at'_n n scptr s \<and> valid_refills_number mrefills n) and
+      ex_nonz_cap_to' scptr and K (MIN_REFILLS \<le> mrefills) and
+      K (budget \<le> MAX_SC_PERIOD \<and> budget \<ge> MIN_SC_BUDGET \<and>
+         period \<le> MAX_SC_PERIOD \<and> budget \<ge> MIN_SC_BUDGET \<and>
+         budget \<le> period))"
+
+primrec sc_inv_rel :: "Invocations_A.sched_context_invocation \<Rightarrow> sched_context_invocation \<Rightarrow> bool"
+  where
+  "sc_inv_rel (Invocations_A.InvokeSchedContextConsumed sc bf) sci' =
+   (sci' = InvokeSchedContextConsumed sc bf)"
+| "sc_inv_rel (Invocations_A.InvokeSchedContextBind sc cap) sci' =
+   (\<exists>cap'. cap_relation cap cap' \<and> sci' = InvokeSchedContextBind sc cap')"
+| "sc_inv_rel (Invocations_A.InvokeSchedContextUnbindObject sc cap) sci' =
+   (\<exists>cap'. cap_relation cap cap' \<and> sci' = InvokeSchedContextUnbindObject sc cap')"
+| "sc_inv_rel (Invocations_A.InvokeSchedContextUnbind sc cap) sci' =
+   (sci' = InvokeSchedContextUnbind sc)" \<comment> \<open>FIXME RT: remove cap in abstract InvokeSchedContextUnbind\<close>
+| "sc_inv_rel (Invocations_A.InvokeSchedContextYieldTo sc bf) sci' =
+   (sci' = InvokeSchedContextYieldTo sc bf)"
+
+primrec sc_ctrl_inv_rel ::
+  "Invocations_A.sched_control_invocation \<Rightarrow> sched_control_invocation \<Rightarrow> bool" where
+  "sc_ctrl_inv_rel (Invocations_A.InvokeSchedControlConfigure sc budget period refills badge) sci' =
+    (sci' = InvokeSchedControlConfigure sc budget period refills badge)"
+
+
+lemma decodeSchedContextInvocation_wf:
+  "\<lbrace> valid_cap' (SchedContextCap sc n) and invs' and sch_act_simple and ex_nonz_cap_to' sc and
+     (\<lambda>s. \<forall>cap\<in>set excaps. \<forall>r\<in>zobj_refs' cap. ex_nonz_cap_to' r s) and
+     (\<lambda>s. \<forall>x\<in>set excaps. valid_cap' x s) \<rbrace>
+   decodeSchedContextInvocation label sc excaps args
+   \<lbrace>valid_sc_inv'\<rbrace>, -"
+  sorry
+
+lemma decodeSchedControlInvocation_wf:
+  "\<lbrace> invs' and sch_act_simple and
+     (\<lambda>s. \<forall>cap\<in>set excaps. \<forall>r\<in>zobj_refs' cap. ex_nonz_cap_to' r s) and
+     (\<lambda>s. \<forall>x\<in>set excaps. valid_cap' x s) \<rbrace>
+   decodeSchedControlInvocation label args excaps
+   \<lbrace>valid_sc_ctrl_inv'\<rbrace>, -"
+  sorry
+
 
 end
 
